Fixes.
Height is now Nat. Proves patterns are complete in rebalances.
Increasing z3rlimit for some functions.

AVL.fst
@@ -3,7 +3,7 @@ open FStar.Tactics
 
 type tree =
      | Leaf : tree
-     | Node : key:int -> l:tree -> r:tree -> ah:int -> tree
+     | Node : key:int -> l:tree -> r:tree -> ah:nat -> tree
 
 val in_tree : x:int -> t:tree -> Tot bool
 let rec in_tree x = function
@@ -29,7 +29,7 @@ let rec is_bst = function
 val max : x:int -> y:int -> Tot (r:int {r = x \/ r = y})
 let max x y = if x > y then x else y
 
-val real_height : t:tree -> Tot int
+val real_height : t:tree -> Tot nat
 
 let rec real_height = function
   | Leaf -> 0
@@ -38,13 +38,13 @@ let rec real_height = function
     let hr = real_height r in
     1 + max hl hr
 
-val node_height : tree -> tree -> Tot int
+val node_height : tree -> tree -> Tot nat
 let node_height l r =
   let hl = real_height l in
   let hr = real_height r in
   1 + max hl hr
 
-val is_real_h : int -> tree -> tree -> Tot bool
+val is_real_h : nat -> tree -> tree -> Tot bool
 let is_real_h v l r = v = node_height l r
 
 val has_real_heights : tree -> Tot bool
@@ -52,12 +52,12 @@ let rec has_real_heights = function
   | Leaf -> true
   | Node _ l r ah -> is_real_h ah l r && has_real_heights l && has_real_heights r
 
-val get_height : t:tree {has_real_heights t} -> Tot (r:int {r = real_height t})
+val get_height : t:tree {has_real_heights t} -> Tot (r:nat {r = real_height t})
 let get_height = function
     |Leaf -> 0
     | Node _ _ _ h -> h
 
-val has_bal : int -> tree -> tree -> Tot bool
+val has_bal : nat -> tree -> tree -> Tot bool
 let has_bal x l r =
   let d = real_height l - real_height r in
   0 - x <= d && d <= x
@@ -94,12 +94,10 @@ let mk_node v l r =
    Node v l r h
 
 val is_empty : t:tree -> Tot bool
-let is_empty = function
-  | Leaf -> true
-  | Node _ _ _ _ -> false
+let is_empty = Leaf?
 
 val not_empty : t:tree -> Tot bool
-let not_empty t = not (is_empty t)
+let not_empty = Node?
 
 val head: t:tree {not_empty t} -> Tot int
 let head (Node x _ _ _) = x
@@ -148,14 +146,14 @@ let all_more_intro v x l r  = ()
 val all_less_intro: v:int -> x:int {x < v} -> l:avll x {all_less_than v l} -> r:avlr x {all_less_than v r && has_bal 1 l r} -> Lemma ((all_less_than v (mk_node x l r)))
 let all_less_intro v x l r  = ()
 
-let impossible = x:int{false}
+// bajo la hipótesis de False, `()` tiene cualquier tipo, en particular `a`
+let unreachable #a () : Pure a (requires False) (ensures (fun _ -> True)) = ()
 
+#push-options "--z3rlimit 25"
 val balL0 : x:int -> l:avll x {is_not_heavy l} -> r:avlr x {is_left_big l r} -> Tot (t:avln (real_height l + 1) {(forall y. in_tree y t <==> in_tree y l \/ in_tree y r \/ x = y)})
-let balL0 x l r = match l with
-  | (Node lv ll lr _) ->
-    let y = mk_node x lr r in
-    mk_node lv ll y
-  | _ -> admit ()
+let balL0 x (Node lv ll lr _) r =
+    mk_node lv ll (mk_node x lr r)
+#pop-options
 
 val balLL : x:int -> l:avll x {is_left_heavy l} -> r:avlr x {is_left_big l r} -> Tot (avlt l)
 let balLL v (Node lv ll lr _) r =
@@ -165,6 +163,9 @@ val eq_or_up : s:tree{has_real_heights s} -> t:tree{has_real_heights t} -> Tot b
 let eq_or_up s t =
   let d = diff t s in
   d = 0 || d = 1
+
+val eq_or_down: s:tree{has_real_heights s} -> t:tree{has_real_heights t} -> Tot bool
+let eq_or_down s t = eq_or_up t s
 
 val bal_ht : l:tree -> r:tree -> t:tree -> Tot bool
 let bal_ht l r t = not (has_bal 1 l r) || is_real_h (real_height t) l r
@@ -180,34 +181,25 @@ let big_ht l r t =
 val re_bal : l:tree {has_real_heights l} -> r:tree {has_real_heights r} -> t:tree{has_real_heights t} -> Tot bool
 let re_bal l r t = big_ht l r t && bal_ht l r t
 
+#push-options "--z3rlimit 25"
+
 val balLR :x:int  -> l:avll x {is_right_heavy l} -> r:avlr x {is_left_big l r} -> Tot (t:avlt l  {(forall y. in_tree y t <==> in_tree y l \/ in_tree y r \/ x = y)})
-let balLR v l r = match l with
-  | (Node lv ll (Node lrv lrl lrr _) lh) ->
-    mk_node lrv (mk_node lv ll lrl) (mk_node v lrr r)
-  | _ ->
-    (* should be impossible *)
-    admit()
+let balLR v (Node lv ll (Node lrv lrl lrr _) lh) r =
+  mk_node lrv (mk_node lv ll lrl) (mk_node v lrr r)
 
 val balR0 : x:int  -> r:avlr x {is_not_heavy r} -> l:avll x {is_right_big l r} -> Tot (t:avln (real_height r + 1) {(forall y. in_tree y t <==> in_tree y l \/ in_tree y r \/ x = y)})
-let balR0 x r l = match r with
-  | (Node rv rl rr _) ->
-    mk_node rv (mk_node x l rl) rr
-  | _ ->
-   (* should be impossible *)
-    admit ()
+let balR0 x (Node rv rl rr _) l =
+  mk_node rv (mk_node x l rl) rr
 
+#pop-options
 
 val balRR : x:int -> l:avll x -> r:avlr x {is_right_big l r && is_right_heavy r} -> Tot (t:avlt r { (forall y. in_tree y t <==> in_tree y l \/ in_tree y r \/ x = y)})
 let balRR x l (Node rv rl rr _) =
   mk_node rv (mk_node x l rl) rr
 
 val balRL : x:int -> l: avll x -> r:avlr x {is_right_big l r && is_left_heavy r} -> Tot (t:avlt r {(forall y. in_tree y t <==> in_tree y l \/ in_tree y r \/ x = y)})
-let balRL x l = function
-  | (Node rv (Node rlv rll rlr _) rr _) ->
+let balRL x l (Node rv (Node rlv rll rlr _) rr _) =
     mk_node rlv (mk_node x l rll ) (mk_node rv rlr rr)
-  | _ ->
-    (* should be impossible *)
-    admit ()
 
 val no_balancing_needed : l:tree {has_real_heights l } -> r:tree {has_real_heights r /\ has_bal 2 l r /\ not (is_left_big l r) /\ not (is_right_big l r)} -> Lemma (has_bal 1 l r)
 let no_balancing_needed l r = ()
@@ -224,79 +216,23 @@ let balance_irb v l r =
   else if (is_right_heavy r) then balRR v l r
   else balR0 v r l
 
-
 val bal : x:int -> l:avll x -> r:avlr x {has_bal 2 l r} -> Tot (t:avl {re_bal l r t /\ (forall y. in_tree y t <==> in_tree y l \/ in_tree y r \/ x = y)})
 let bal v l r  =
-  let ilb = is_left_big l r in
-  let irb = is_right_big l r in
-  if (ilb) then balance_ilb v l r
-  else if (irb) then balance_irb v l r
+  if (is_left_big l r) then balance_ilb v l r
+  else if (is_right_big l r) then balance_irb v l r
   else begin
     no_balancing_needed l r;
     mk_node v l r
   end
 
-
-val in_tree_less_than_lemma : v:int -> t:tree {forall y. (in_tree y t ==> y < v)} -> Lemma (all_less_than v t)
-let in_tree_less_than_lemma v t = ()
-
-
-val in_tree_more_than_lemma : v:int -> t:tree {forall y. (in_tree y t ==> y > v)} -> Lemma (all_more_than v t)
-let in_tree_more_than_lemma v t = ()
-
-
-val less_than_in_tree_lemma : v:int -> t:tree {all_less_than v t} -> Lemma (forall y. (in_tree y t ==> y < v))
-let less_than_in_tree_lemma v t = ()
-
-
-val more_than_in_tree_lemma : v:int -> t:tree {all_more_than v t} -> Lemma (forall y. (in_tree y t ==> y > v))
-let more_than_in_tree_lemma v t = ()
-
-val bal_not_empty : x:int -> l:avll x -> r:avlr x {has_bal 2 l r} -> Lemma (not_empty (bal x l r))
-let bal_not_empty x l r = ()
-
-val bal_height : x:int -> l:avll x -> r:avlr x {has_bal 2 l r} -> Lemma (real_height (bal x l r) = node_height l r \/ real_height (bal x l r) = node_height l r - 1)
-let bal_height x l r = ()
-
-val bal_in_tree : x:int -> l:avll x -> r:avlr x {has_bal 2 l r} -> Lemma (forall y. in_tree y (bal x l r) <==> in_tree y l \/ in_tree y r \/ x = y)
-let bal_in_tree x l r = ()
-
-val intro_diff_0_or_1_c :t:tree -> s:tree {real_height t - real_height s >= 0 /\ real_height t - real_height s <= 1} -> Lemma (real_diff t s = 0 \/ real_diff t s = 1)
-let intro_diff_0_or_1_c t s = ()
-
 val insert: x:int -> s:avl -> Tot (t:avl {not_empty t /\ eq_or_up s t /\ (forall y. (in_tree y t) <==> (in_tree y s \/ x = y))})
+#push-options "--z3rlimit 50"
 let rec insert x s = match s with
   | Leaf -> singleton x
   | Node v l r _ ->
     if x < v then begin
-      let insl = insert x l in
-      less_than_in_tree_lemma v l;
-      in_tree_less_than_lemma v insl;
-      bal_not_empty v insl r;
-      bal_height v insl r;
-      bal_in_tree v insl r;
-      intro_diff_0_or_1_c (bal v insl r) s;
-      assert (forall y. (in_tree y (bal v insl r)) <==> (in_tree y s \/ x = y));
-      assert (not_empty (bal v insl r));
-      assert (eq_or_up s (bal v insl r));
-      bal v insl r
+      bal v (insert x l) r
     end else if x > v then begin
-      let insr = insert x r in
-      more_than_in_tree_lemma v r;
-      in_tree_more_than_lemma v insr;
-      bal_not_empty v l insr;
-      bal_height v l insr;
-      bal_in_tree v l insr;
-      (assert (forall y. in_tree y insr <==> in_tree y r \/ x = y));
-      in_tree_more_than_lemma v insr;
-      intro_diff_0_or_1_c (bal v l insr) s;
-      assert (eq_or_up s (bal v l insr));
-      assert (not_empty (bal v l insr));
-      assert (forall y. (in_tree y s) <==> in_tree y l \/ in_tree y r \/ v = y);
-
-      assert (forall y. (in_tree y (bal v l insr)) <==> (in_tree y l \/ in_tree y r \/ v = y \/ x = y));
-      assert (forall y. (in_tree y (bal v l insr)) <==> (in_tree y s \/ x = y));
-      assert (not_empty (bal v l insr));
-      assert (eq_or_up s (bal v l insr));
-      bal v l insr
+      bal v l (insert x r)
     end else s
+#pop-options
